theories/rust_typing/ltype_rules.v
@@ -832,17 +832,3 @@ Section guarded.
     by apply Hle.
   Qed.
 End guarded.
-
-(** extend [solve_type_proper] *)
-Ltac solve_type_proper_hook ::=
-  match goal with
-    | |- ltype_own (OfTy _) ?bk _ _ _ ≡{_}≡ ltype_own (OfTy _) ?bk _ _ _ =>
-      match bk with
-      | Shared _ => apply ofty_own_ne_shared; try apply _
-      | Uniq _ _ => apply ofty_own_contr_uniq; try apply _
-      | Owned true => apply ofty_own_contr_owned; try apply _
-      | Owned false => apply ofty_own_ne_owned; try apply _
-      end
-    | |- guarded _ ≡{_}≡ guarded _ =>
-      apply guarded_dist; iIntros
-  end.
