theories/rust_typing/typing.v
@@ -1,7 +1,7 @@
 From refinedrust Require Export static type program_rules int int_rules unit struct.struct mut_ref.mut_ref shr_ref.shr_ref functions uninit box programs enum maybe_uninit alias_ptr fixpoint existentials existentials_na array.array value generics xmap.
 From refinedrust Require Export automation.loc_eq manual automation.
 From iris.proofmode Require Import coq_tactics reduction string_ident.
-From refinedrust Require Export simpl.
+From refinedrust Require Export automation.simpl.
 From refinedrust Require Export options.
 
 (* In my experience, this has led to more problems with [normalize_autorewrite] rewriting below definitions too eagerly. *)
